added assumption to sscanleqlemma

src/demo/flasher/NotAutomat.thy
@@ -13,23 +13,13 @@ interpretation not_smap:smapGen "dAnot_transition" Single "buildNotinSBE" "build
   apply auto[1]
   done
 
+definition "notStrong  \<equiv>  (dAutomaton_weak.extend not_smap.da (dAutomaton_strong.fields (notOutSBE.setter True)))"
+
 abbreviation notStep::"(S_not \<Rightarrow> (inNot\<^sup>\<Omega> \<rightarrow> outNot\<^sup>\<Omega>))"where
 "notStep \<equiv> dawStateSem not_smap.da"
 
 definition notSpf::"(inNot\<^sup>\<Omega> \<rightarrow> outNot\<^sup>\<Omega>)"where
-"notSpf = dasSem (dAutomaton_weak.extend not_smap.da (dAutomaton_strong.fields (notOutSBE.setter True)))"
-
-
-lemma dasinitout_well:"(dasInitOut
-         (dAutomaton_weak.extend daw
-           (dAutomaton_strong.fields
-             sbe))) = sbe" (*How proof this?*)
-  sorry
-
-lemma das2daw_trunc_well:"dAutomaton_weak.truncate
-                (dAutomaton_weak.extend da
-                  (dAutomaton_strong.fields sbe)) = da" (*How proof this?*)
-  sorry
+"notSpf = dasSem notStrong"
 
 lemma notingetset_eq:"notInSBE.getterSB\<cdot>(notInSBE.setterSB\<cdot>s) = s"
   by(simp)
@@ -38,13 +28,10 @@ lemma notoutgetset_eq:"notOutSBE.getterSB\<cdot> (notOutSBE.setterSB\<cdot>s) = 
   by(simp)
 
 lemma notstep2smap:"notOutSBE.getterSB\<cdot>(notStep state\<cdot>(notInSBE.setterSB\<cdot>input)) = (smap not_smap.smapTransition)\<cdot>input"
-  by (metis (full_types) S_not.exhaust not_smap.daut2smap)
-
-thm dAutomaton_weak.select_convs
-
+  by (metis (mono_tags, lifting) S_not.exhaust not_smap.daut2smap somechannotempty)
 
 lemma "notOutSBE.getterSB\<cdot>(notSpf\<cdot>(notInSBE.setterSB\<cdot>input)) = \<up>True \<bullet>(smap not_smap.smapTransition)\<cdot>input"
-  by(simp add: notSpf_def dasSem_def dasinitout_well das2daw_trunc_well dawSem_def notstep2smap)
+  by(simp add: notSpf_def dasSem_def dasinitout_well das2daw_trunc_well dawSem_def notstep2smap notStrong_def)
 
 lemma not_step:"smap not_smap.smapTransition\<cdot>(\<up>bool \<bullet> s) = \<up>(\<not>bool) \<bullet> smap not_smap.smapTransition\<cdot>s"
   by simp
